Prove soundness of tree-proof checker

src/named/TreeProofs.v
@@ -35,6 +35,54 @@ Section WithVar.
     (wf_ctx (Model:= core_model l)).
 
   
+    (*TODO: backport these to core.v?*)
+    
+    Lemma term_con_congruence l c t name s1 s2 c' args t'
+      : In (name, term_rule c' args t') l ->
+        t = t'[/with_names_from c' s2/] ->
+        wf_lang l ->
+        eq_args l c c' s1 s2 ->
+        eq_term l c t (con name s1) (con name s2).
+    Proof.
+      intros.
+      assert (wf_ctx l c') by with_rule_in_wf_crush.
+      rewrite <- (wf_con_id_args_subst c' s1);[| basic_core_crush..].
+      rewrite <- (wf_con_id_args_subst c' s2);[|basic_core_crush..].
+      subst.
+      change (con ?n ?args[/?s/]) with (con n args)[/s/].
+      eapply eq_term_subst; eauto.
+      {
+        apply eq_args_implies_eq_subst; eauto.
+      }
+      {
+        constructor.
+        replace t' with t'[/id_subst c'/].
+        - eapply wf_term_by; basic_core_crush.
+        - basic_core_crush.
+      }
+    Qed.
+    
+    Lemma sort_con_congruence l c name s1 s2 c' args
+      : In (name, sort_rule c' args) l ->
+        wf_lang l ->
+        eq_args l c c' s1 s2 ->
+        eq_sort l c (scon name s1) (scon name s2).
+    Proof.
+      intros.
+      assert (wf_ctx l c') by with_rule_in_wf_crush.
+      rewrite <- (wf_con_id_args_subst c' s1);[| basic_core_crush..].
+      rewrite <- (wf_con_id_args_subst c' s2);[|basic_core_crush..].
+      subst.
+      change (scon ?n ?args[/?s/]) with (scon n args)[/s/].
+      eapply eq_sort_subst; eauto.
+      { apply eq_args_implies_eq_subst; eauto. }
+      { constructor.
+        eapply wf_sort_by; basic_core_crush.
+      }
+    Qed.
+
+
+  
   (* The type doesn't discriminate between term and sort equalities *)
   Unset Elimination Schemes.
   Inductive pf : Type :=
@@ -110,11 +158,6 @@ Section WithVar.
         (forall p1 : pf, P p1 -> forall p2 : pf, P p2 -> P (ptrans p1 p2)) ->
         (forall p : pf, P p -> P (psym p)) ->
         (forall p1 : pf, P p1 -> forall p2 : pf, P p2 -> P (pconv p1 p2)) -> forall e : pf, P e.
-
-  Variant pf_fact :=
-    | tm_eq (e1 : term) (e2 : term) (t : sort)
-    | srt_eq (t1:sort) (t2:sort).
-
   
 
   Section WithLang.
@@ -124,59 +167,198 @@ Section WithVar.
     Context (c : ctx).
 
     Section Inner.
-      Context (check_proof : pf -> option pf_fact).
+      Context (check_proof : pf -> option (term * term * sort)).
       Fixpoint check_args_proof (args : list pf) (c' : ctx) :=
         match args, c' with
         | [], [] => Some ([],[])
         | p::args, (_,t)::c'=>
             @! let (lhs, rhs) <- check_args_proof args c' in
-               let (tm_eq e1 e2 t') <?- check_proof p in
+               let (e1, e2, t') <- check_proof p in
                (*TODO: use Eqb instance*)
-               let ! sort_eq_dec t[/with_names_from c' lhs/] t' in
+               let ! sort_eq_dec t[/with_names_from c' rhs/] t' in
                ret (e1::lhs, e2::rhs)
         | _,_=> None
         end.
     End Inner.
     
-    (*TODO: split fn by output*)
-    Fixpoint check_proof (p : pf) : option pf_fact :=
+    Fixpoint check_proof (p : pf) : option (term * term * sort) :=
       match p with
       | pvar n =>
           @! let t <- named_list_lookup_err c n in
-             ret tm_eq (var n) (var n) t
+             ret (var n, var n, t)
+      | pcon n s =>
+          @! let r <- named_list_lookup_err l n in
+             match r with
+             | term_rule c' _ t =>
+                 @! let (lhs, rhs) <- check_args_proof check_proof s c' in
+                    ret (con n lhs, con n rhs, t[/with_names_from c' rhs/])
+             | term_eq_rule c' e1 e2 t =>
+                 @! let (lhs, rhs) <- check_args_proof check_proof s c' in
+                    let lsub := with_names_from c' lhs in
+                    let rsub := with_names_from c' rhs in
+                    ret (e1[/lsub/],e2[/rsub/],t[/rsub/])
+             | _ => None
+             end
+      | ptrans p0 p1 =>
+          @! let (e1, e2, t) <- check_proof p0 in
+             let (e1', e2', t') <- check_proof p1 in
+             let ! sort_eq_dec t t' in
+             let ! term_eq_dec e2 e1' in
+             ret (e1, e2', t)
+      | psym p =>
+          @! let (e1, e2, t) <- check_proof p in
+             ret (e2, e1, t)
+      | pconv p0 p1 =>
+          @! let (t1, t2) <- check_sort_proof p0 in
+             let (e1, e2, t) <- check_proof p1 in
+             let ! sort_eq_dec t t1 in
+             ret (e1, e2, t2)
+      end
+    
+    with check_sort_proof (p : pf) : option (sort * sort) :=
+      match p with
+      | pvar n => None
       | pcon n s =>
           @! let r <- named_list_lookup_err l n in
              match r with
              | sort_rule c' _ =>
                  @! let (lhs, rhs) <- check_args_proof check_proof s c' in
-                    ret srt_eq (scon n lhs) (scon n rhs)
-             | term_rule c' _ t =>
-                 @! let (lhs, rhs) <- check_args_proof check_proof s c' in
-                    ret tm_eq (con n lhs) (con n rhs) t[/with_names_from c' lhs/]
+                    ret (scon n lhs, scon n rhs)
              | sort_eq_rule c' t1 t2 =>
                  @! let (lhs, rhs) <- check_args_proof check_proof s c' in
                     let lsub := with_names_from c' lhs in
                     let rsub := with_names_from c' rhs in
-                    ret srt_eq t1[/lsub/] t2[/rsub/]
-             | term_eq_rule c' e1 e2 t =>
-                 @! let (lhs, rhs) <- check_args_proof check_proof s c' in
-                    let lsub := with_names_from c' lhs in
-                    let rsub := with_names_from c' rhs in
-                    ret tm_eq e1[/lsub/] e2[/rsub/] t[/lsub/]
+                    ret (t1[/lsub/], t2[/rsub/])
+             | _ => None
              end
-               (*TODO: needs to run on sort eqs*)
       | ptrans p0 p1 =>
-          @! let (tm_eq e1 e2 t) <?- check_proof p0 in
-             let (tm_eq e1' e2' t') <?- check_proof p1 in
-             let ! sort_eq_dec t t' in
-             let ! term_eq_dec e2 e1' in
-             ret tm_eq e1 e2' t
+          @! let (t1, t2) <- check_sort_proof p0 in
+             let (t1', t2') <- check_sort_proof p1 in
+             let ! sort_eq_dec t2 t1' in
+             ret (t1, t2')
       | psym p =>
-          @! let (tm_eq e1 e2 t) <?- check_proof p in
-             ret (tm_eq e2 e1 t)
-      | pconv p0 p1 =>
-          @! let (tm_eq e1 e2 t) <?- check_proof p0 in
-             let (srt_eq t1 t2) <?- check_proof p1 in
-             let ! sort_eq_dec t t1 in
-             ret tm_eq e1 e2 t2
+          @! let (t1,t2) <- check_sort_proof p in
+             ret (t2,t1)
+      | pconv _ _ => None
       end.
+
+    Context (wfl : wf_lang l)
+            (wfc : wf_ctx l c).
+
+    
+  (*TOOD: replace case_match with this? Copied once already*)
+  Ltac case_match' :=
+    try lazymatch goal with
+          [ H :  context [ match ?e with
+                           | _ => _
+                           end] |- _ ] => revert H
+        end;
+    case_match.
+
+
+    
+    Lemma pf_checker_sound p
+      : (forall t1 t2,
+        check_sort_proof p = Some (t1, t2) ->
+        eq_sort l c t1 t2)
+    /\ (forall t e1 e2,
+           check_proof p = Some (e1, e2, t) ->
+           eq_term l c t e1 e2).
+    Proof.
+      induction p;
+        split;
+        basic_goal_prep;
+        (*weed out trivial goals for efficiency*)
+        try congruence;
+        repeat case_match';
+        basic_goal_prep;
+        try congruence;
+        repeat lazymatch goal with
+        | [H : Some _ = Some _ |- _ ] => safe_invert H
+               end.
+      - constructor; constructor.
+        eapply named_list_lookup_err_in; eauto.
+      - safe_invert HeqH3.
+        eapply sort_con_congruence; eauto.
+        + eapply named_list_lookup_err_in; eauto.
+        + {
+            clear HeqH0.
+            revert H c0 l4 l5 HeqH2.
+            induction l0;
+              basic_goal_prep;
+              repeat case_match';
+              try congruence;
+              basic_goal_prep;
+              basic_core_crush.
+            constructor; eauto.
+            eapply H2; auto.
+          }
+      - safe_invert HeqH3.
+        eapply eq_sort_subst; cycle 2.
+        + basic_core_crush.
+        + with_rule_in_wf_crush.
+        + clear HeqH0.
+          revert H c0 l3 l4 HeqH2.
+          induction l0;
+            basic_goal_prep;
+            repeat case_match';
+            try congruence;
+            basic_goal_prep;
+            basic_core_crush.
+          constructor; eauto.
+          eapply H2; auto.
+      - safe_invert HeqH3.
+        eapply term_con_congruence; eauto.
+        + eapply named_list_lookup_err_in; eauto.
+        + {
+            clear HeqH0.
+            revert H c0 l4 l5 HeqH2.
+            induction l0;
+              basic_goal_prep;
+              repeat case_match';
+              try congruence;
+              basic_goal_prep;
+              basic_core_crush.
+            constructor; eauto.
+            eapply H2; auto.
+          }
+      - safe_invert HeqH3.
+        eapply eq_term_subst; cycle 2.
+        + basic_core_crush.
+        + with_rule_in_wf_crush.
+        + clear HeqH0.
+          revert H c0 l3 l4 HeqH2.
+          induction l0;
+            basic_goal_prep;
+            repeat case_match';
+            try congruence;
+            basic_goal_prep;
+            basic_core_crush.
+          constructor; eauto.
+          eapply H2; auto.
+      - safe_invert HeqH2.
+        eapply eq_sort_trans; eauto.
+      - inversion H.
+      - autorewrite with utils in *.
+        intuition subst.
+        eapply eq_term_trans; eauto.
+      - autorewrite with utils in *.
+        intuition subst.
+      - autorewrite with utils in *.
+        intuition subst.
+      - autorewrite with utils in *.
+        intuition subst.
+        eapply eq_sort_sym; eauto.
+      - autorewrite with utils in *.
+        intuition subst.
+        eapply eq_term_sym; eauto.
+      - autorewrite with utils in *.
+        intuition subst.
+        eapply eq_term_conv; eauto.
+      - autorewrite with utils in *.
+        intuition subst.
+    Qed.
+
+    End WithLang.
+  
+End WithVar.
